Update Sorting_Pairwise_Sums.thy

Sorting_Pairwise_Sums.thy
@@ -1,16 +1,16 @@
 theory "Sorting_Pairwise_Sums"
-  imports Main
+  imports Main "HOL-Library.Multiset"
 begin
 
 (* Author: Nemanja Rsumovic 91/2020 *)
 
-definition operation :: "int \<Rightarrow> int \<Rightarrow> int" ("\<oplus>") where
-  "\<oplus> x y = x + y"
+definition operation :: "int ⇒ int ⇒ int" ("⊕") where
+  "⊕ x y = x + y"
 
 (* Pairwise sums function: computes all pairwise sums of two lists *)
-fun pairwise_sums :: "int list \<Rightarrow> int list \<Rightarrow> int list" where
+fun pairwise_sums :: "int list ⇒ int list ⇒ int list" where
   "pairwise_sums [] _ = []" |
-  "pairwise_sums (x#xs) ys = (map (\<lambda>y. \<oplus> x y) ys) @ (pairwise_sums xs ys)"
+  "pairwise_sums (x#xs) ys = (map (λy. ⊕ x y) ys) @ (pairwise_sums xs ys)"
 
 value "pairwise_sums [1,2] [3,4]"            (* Expected result: [4, 5, 5, 6] *)
 value "pairwise_sums [1,2,3] [1000,100,10]"  (* Expected result: [1001, 101, 11, 1002, 102, 12, 1003, 103, 13] *)
@@ -29,7 +29,7 @@ value "pairwise_sums [] [3,4]"
 value "pairwise_sums [1,2] []"
 
 (* Sorting the pairwise sums *)
-definition sortsums :: "int list \<Rightarrow> int list \<Rightarrow> int list" where
+definition sortsums :: "int list ⇒ int list ⇒ int list" where
   "sortsums xs ys = sort (pairwise_sums xs ys)"
 
 value "sortsums [1,2] [3,4]"            (* Expected result: [4, 5, 5, 6] *)
@@ -62,35 +62,35 @@ lemma sortsums_complexity:
   by (simp add: sortsums_size)
  
 theorem sorting_pairwise_sums_correct:
-  "sorted (sortsums xs ys) \<and> length (sortsums xs ys) = length xs * length ys"
+  "sorted (sortsums xs ys) ∧ length (sortsums xs ys) = length xs * length ys"
   by (simp add: sortsums_sorted sortsums_size)
 
 (*<---------------------- Lambert’s algorithm ---------------------->*)
 
-definition negate :: "int \<Rightarrow> int" where
+definition negate :: "int ⇒ int" where
   "negate x = - x"
 
-definition operation_negate :: "int \<Rightarrow> int \<Rightarrow> int" ("\<ominus>") where
-  "\<ominus> x y = \<oplus> x (negate y)"
+definition operation_negate :: "int ⇒ int ⇒ int" ("⊖") where
+  "⊖ x y = ⊕ x (negate y)"
 
 (* Generate a list of indices with the same length as the list xs *)
-definition zip_with_indices :: "int list \<Rightarrow> (int \<times> nat) list" where
+definition zip_with_indices :: "int list ⇒ (int × nat) list" where
   "zip_with_indices xs = zip xs (upt 1 (length xs + 1))"
 
 value "zip_with_indices [5,6,7]"  (* Expected result: [(5,1), (6,2), (7,3)] *)
 
 
 (* Function that generates a list of pairs with indices and subs their values *)
-fun subs :: "int list \<Rightarrow> int list \<Rightarrow> (int \<times> (nat \<times> nat)) list" where
+fun subs :: "int list ⇒ int list ⇒ (int × (nat × nat)) list" where
   "subs [] _ = []"
 | "subs _ [] = []"
 | "subs xs ys=
         concat(
                         map (
-                               \<lambda> (x, i). 
+                               λ (x, i). 
                               map (
-                                    \<lambda> (y, j). 
-                                    (\<ominus> x y, (i, j))) 
+                                    λ (y, j). 
+                                    (⊖ x y, (i, j))) 
                                     (zip_with_indices ys)) 
                               (zip_with_indices xs)
                 )"
@@ -98,14 +98,18 @@ fun subs :: "int list \<Rightarrow> int list \<Rightarrow> (int \<times> (nat \<
 value "subs [7, 12] [4, 6]"  (* Expected result: [(3, (1, 1)), (1, (1, 2)), (8, (2, 1)), (6, (2, 2))] *)
 
 (* General merge function that accepts a comparison function *)
-fun merge :: "('a::ord \<times> 'b) list \<Rightarrow> ('a \<times> 'b) list \<Rightarrow> ('a \<times> 'b) list"
+fun merge :: "('a::ord × 'b) list ⇒ ('a × 'b) list ⇒ ('a × 'b) list"
   where
     "merge [] ys = ys" |
     "merge xs [] = xs" |
-    "merge (x#xs) (y#ys) = (if fst x \<le> fst y then x # merge xs (y#ys) else y # merge (x#xs) ys)"
+    "merge (x#xs) (y#ys) = 
+      (if fst x ≤ fst y then 
+          x # merge xs (y#ys)
+      else
+          y # merge (x#xs) ys)"
 
 (* Divide and Conquer method for sorting the subs using  merge *)
-fun sortsubs' :: "(int \<times> (nat \<times> nat)) list \<Rightarrow> (int \<times> (nat \<times> nat)) list" where
+fun sortsubs' :: "(int × (nat × nat)) list ⇒ (int × (nat × nat)) list" where
   "sortsubs' [] = []" |
   "sortsubs' [x] = [x]" |
   "sortsubs' xs = (
@@ -116,42 +120,80 @@ fun sortsubs' :: "(int \<times> (nat \<times> nat)) list \<Rightarrow> (int \<ti
   )"
 
 (* Sorting the subs *)
-definition sortsubs :: "int list \<Rightarrow> int list \<Rightarrow> (int \<times> (nat \<times> nat)) list" where
+definition sortsubs :: "int list ⇒ int list ⇒ (int × (nat × nat)) list" where
   "sortsubs xs ys = sortsubs' (subs xs ys)"
 
 value "sortsubs [7, 12] [4, 6]"            (* Expected result: [(1, (1, 2)), (3, (1, 1)), (6, (2, 2)), (8, (2, 1))] *)
 value "map fst (sortsubs [7, 12] [4, 6])"  (* Expected result: [1, 3, 6, 8] *)
 
-(* Lemma: Sorting preserves the length of the list *)
-lemma sorted_size_preserved2[simp]:
-  shows "length (sortsubs xs ys) = length (subs xs ys)"
-  proof -
-  have "sortsubs xs ys = sortsubs' (subs xs ys)"
-    by (simp add: sortsubs_def)
-  then show ?thesis
-    by (induction "subs xs ys" rule: sortsubs'.induct, auto)
+definition f_subs ::  "int list ⇒ int list ⇒ int list" where
+  "f_subs xs ys = map fst (subs xs ys)"
+
+definition f_sortsubs ::  "int list ⇒ int list ⇒ int list" where
+  "f_sortsubs xs ys = map fst (sortsubs xs ys)"
+
+value "f_subs [7,12] [4,6]"
+value "f_sortsubs [7,12] [4,6]"
+
+(*<----------------------------------------------------------------->*)
+(* Lemma: sortsubs' returns a sorted list *)
+lemma merge_mset[simp]:
+  shows "mset (merge xs ys) = mset xs + mset ys"
+  apply (induction xs ys rule: merge.induct)
+    apply auto
+  done
+
+lemma merge_set[simp]:
+  shows "set (merge xs ys) = set xs ∪ set ys"
+  apply (induction xs ys rule: merge.induct)
+    apply auto
+  done
+
+lemma sortedMerge[simp]:
+  assumes "sorted (map fst xs)" "sorted (map fst ys)"
+  shows "sorted (map fst (merge xs ys))"
+  using assms
+  apply (induction xs ys rule: merge.induct)
+    apply auto
+  done
+
+lemma sortsubs'_sorted:
+  shows "sorted (map fst (sortsubs' xs))"
+proof (induction xs rule: sortsubs'.induct)
+  case 1
+  then show ?case by auto
+next
+  case (2 x)
+  then show ?case by auto
+next
+  case (3 x0 x1 xs)
+  define mid where "mid = length (x0 # x1 # xs) div 2"
+  define left where "left = take mid (x0 # x1 # xs)"
+  define right where "right = drop mid (x0 # x1 # xs)"
+  have "sortsubs' (x0 # x1 # xs) =  merge (sortsubs' left) (sortsubs' right)"
+    unfolding mid_def left_def right_def
+    by simp
+  moreover
+  have "sorted (map fst (sortsubs' left))"
+    using 3(1) 
+    unfolding mid_def left_def right_def
+    by auto
+  moreover
+  have "sorted (map fst (sortsubs' right))"
+    using 3(2)
+    unfolding mid_def left_def right_def
+    by auto
+  ultimately
+  show ?case 
+    by simp
 qed
 
 (* Lemma: sortsubs returns a sorted list *)
 lemma sortsubs_sorted[simp]:
   shows "sorted (map fst (sortsubs xs ys))"
-  proof -
-  have "sortsubs xs ys = sortsubs' (subs xs ys)"
-    by (simp add: sortsubs_def)
-  then show ?thesis
-  by (induction "subs xs ys" rule: sortsubs'.induct, auto)
-qed
+  unfolding sortsubs_def
+  by (auto simp add: sortsubs'_sorted)
 
-(* Lemma: The length of the result is the product of the lengths of the input lists *)
-lemma sortsubs_size[simp]:
-  shows "length (sortsubs xs ys) = length xs * length ys"
- proof -
-  have "length (subs xs ys) = length xs * length ys"
-    by (induction "subs xs ys" rule: sortsubs'.induct, auto)
-  thus ?thesis
-    by auto
-    qed
-    
 (*<----------------------------------------------------------------->*)
 
 value "sortsums [5,6,7] [10,20,30]"                         (* Expected result: [15, 16, 17, 25, 26, 27, 35, 36, 37] *)
@@ -165,13 +207,13 @@ lemma sortsums_sortsubs:
   
 (*<----------------------------------------------------------------->*)
 
-type_synonym n3 = "(nat \<times> nat \<times> nat)"
+type_synonym n3 = "(nat × nat × nat)"
 
 (* Merging two sorted lists with tags *)
-fun tag :: "nat \<Rightarrow> (int \<times> (nat \<times> nat)) \<Rightarrow> (int \<times> n3)"
+fun tag :: "nat ⇒ (int × (nat × nat)) ⇒ (int × n3)"
   where "tag i (x, (j, k)) = (x, (i, j, k))"
 
-fun table :: "int list \<Rightarrow> int list \<Rightarrow> (nat \<times> nat \<times> nat) list"
+fun table :: "int list ⇒ int list ⇒ (nat × nat × nat) list"
   where "table xs ys = map snd (merge (map (tag 1) (sortsubs xs xs)) (map (tag 2) (sortsubs ys ys)))"
 
   
@@ -183,13 +225,13 @@ mkArray xs ys = array b (zip (table xs ys) [1..])
                       p = max (length xs) (length ys)
 *)
 
-definition p :: "int list \<Rightarrow> int list \<Rightarrow> nat" where
+definition p :: "int list ⇒ int list ⇒ nat" where
   "p xs ys = max (length xs) (length ys)"
 
-definition mkArray_bounds :: "int list \<Rightarrow> int list => (n3 \<times> n3)" where
+definition mkArray_bounds :: "int list ⇒ int list => (n3 × n3)" where
   "mkArray_bounds xs ys = ((1,1,1),(2,(p xs ys),(p xs ys)))"
   
-definition mkArray_zip :: "int list \<Rightarrow> int list \<Rightarrow> (n3 \<times> nat) list" where
+definition mkArray_zip :: "int list ⇒ int list ⇒ (n3 × nat) list" where
   "mkArray_zip xs ys = zip (table xs ys) (map Suc (upt 0 (length (table xs ys))))"
 
 value "table [1,2,3] [4,5]"
@@ -197,30 +239,30 @@ value "mkArray_bounds [1,2,3] [4,5]"
 value "mkArray_zip [1,2,3] [4,5]"
 
 (* Function that checks if (x, y, z) is within bounds *)
-fun in_bounds :: "n3 \<Rightarrow> n3 \<Rightarrow> n3 \<Rightarrow> bool" where
+fun in_bounds :: "n3 ⇒ n3 ⇒ n3 ⇒ bool" where
   "in_bounds (low1, low2, low3) (high1, high2, high3) (x, y, z) =
-    (low1 \<le> x \<and> x \<le> high1 \<and>
-     low2 \<le> y \<and> y \<le> high2 \<and>
-     low3 \<le> z \<and> z \<le> high3)"
+    (low1 ≤ x ∧ x ≤ high1 ∧
+     low2 ≤ y ∧ y ≤ high2 ∧
+     low3 ≤ z ∧ z ≤ high3)"
 
 (* Auxiliary function that filters the list *)
-fun filter_in_bounds :: "n3 \<times> n3 \<Rightarrow> (n3 \<times> nat) list \<Rightarrow> (n3 * nat) list" where
+fun filter_in_bounds :: "n3 × n3 ⇒ (n3 × nat) list ⇒ (n3 * nat) list" where
   "filter_in_bounds bounds [] = []" |
   "filter_in_bounds bounds (((x, y, z), v) # xs) =
      (if in_bounds (fst bounds) (snd bounds) (x, y, z) then ((x, y, z), v) # filter_in_bounds bounds xs
       else filter_in_bounds bounds xs)"
 
 (* Auxiliary function for comparing two elements of type (nat * nat * nat) *)
-fun compare_tuples :: "n3 \<Rightarrow> n3 \<Rightarrow> bool" where
-  "compare_tuples (x1, y1, z1) (x2, y2, z2) = (if x1 < x2 then True else if x1 = x2 then (if y1 < y2 then True else if y1 = y2 then z1 \<le> z2 else False) else False)"
+fun compare_tuples :: "n3 ⇒ n3 ⇒ bool" where
+  "compare_tuples (x1, y1, z1) (x2, y2, z2) = (if x1 < x2 then True else if x1 = x2 then (if y1 < y2 then True else if y1 = y2 then z1 ≤ z2 else False) else False)"
 
 (* Function for sorting the list *)
-fun sort_array :: "(n3 \<times> nat) list \<Rightarrow> (n3 \<times> nat) list" where
+fun sort_array :: "(n3 × nat) list ⇒ (n3 × nat) list" where
   "sort_array [] = []" |
-  "sort_array (x#xs) = sort_array [y \<leftarrow> xs. compare_tuples (fst y) (fst x)] @ [x] @ sort_array [y \<leftarrow> xs. \<not>compare_tuples (fst y) (fst x)]"
+  "sort_array (x#xs) = sort_array [y ← xs. compare_tuples (fst y) (fst x)] @ [x] @ sort_array [y ← xs. ¬compare_tuples (fst y) (fst x)]"
 
 (* The main mkArray function *)
-fun mkArray :: "int list \<Rightarrow> int list \<Rightarrow> (n3 \<times> nat) list" where
+fun mkArray :: "int list ⇒ int list ⇒ (n3 × nat) list" where
   "mkArray xs ys = sort_array (filter_in_bounds (mkArray_bounds xs ys) (mkArray_zip xs ys))"
   
 (* Testing the mkArray function with inputs *)
@@ -239,18 +281,18 @@ cmp a (x,(i,j)) (y,(k,l))
 *)
 value "map_of (mkArray [1,2,3] [4,5])"
 
-fun indexing :: "(n3 \<Rightarrow> nat option) \<Rightarrow> n3 \<Rightarrow> nat" (infix "!!" 105) where
+fun indexing :: "(n3 ⇒ nat option) ⇒ n3 ⇒ nat" (infix "!!" 105) where
   "a !! idx = the (a idx)"
 
 datatype ordering = LT | EQ | GT
 
-fun compare :: "nat \<Rightarrow> nat \<Rightarrow> ordering" where
-  "compare x y = (if x \<le> y then LT else if x > y then GT else EQ)"
+fun compare :: "nat ⇒ nat ⇒ ordering" where
+  "compare x y = (if x ≤ y then LT else if x > y then GT else EQ)"
 
-fun cmp' :: "(n3 \<Rightarrow> nat option) \<Rightarrow> int \<times> nat \<times> nat \<Rightarrow> int \<times> nat \<times> nat \<Rightarrow> ordering" where
+fun cmp' :: "(n3 ⇒ nat option) ⇒ int × nat × nat ⇒ int × nat × nat ⇒ ordering" where
   "cmp' a (x,(i,j)) (y,(k,l)) = compare (a !! (1,i,k)) (a !! (2,j,l))"
 
-fun cmp :: "(n3 \<times> nat) list \<Rightarrow> int \<times> nat \<times> nat \<Rightarrow> int \<times> nat \<times> nat \<Rightarrow> ordering" where
+fun cmp :: "(n3 × nat) list ⇒ int × nat × nat ⇒ int × nat × nat ⇒ ordering" where
   "cmp a (x,(i,j)) (y,(k,l)) = cmp' (map_of a) (x,(i,j)) (y,(k,l))"
   
 value "indexing (map_of (mkArray [1,2,3] [4,5])) (1, 3, 1)"
@@ -258,15 +300,15 @@ value "(map_of (mkArray [1,2,3] [4,5])) !! (1, 3, 1)"
 value "cmp (mkArray [1,2,3] [4,5]) (2, 1, 2) (2, 1, 2) "
 value "mkArray [1,2,3] [4,5]"
 
-fun insert :: "(n3 \<times> nat) list \<Rightarrow> (int \<times> (nat \<times> nat)) \<Rightarrow> (int \<times> (nat \<times> nat)) list \<Rightarrow> (int \<times> (nat \<times> nat)) list" where
+fun insert :: "(n3 × nat) list ⇒ (int × (nat × nat)) ⇒ (int × (nat × nat)) list ⇒ (int × (nat × nat)) list" where
   "insert a x [] = [x]" |
   "insert a x (y#ys) = (if cmp a x y = LT then x # y # ys else y # insert a x ys)"
 
-fun sortsubs2_manual :: "(n3 \<times> nat) list \<Rightarrow> (int \<times> (nat \<times> nat)) list \<Rightarrow> (int \<times> (nat \<times> nat)) list" where
+fun sortsubs2_manual :: "(n3 × nat) list ⇒ (int × (nat × nat)) list ⇒ (int × (nat × nat)) list" where
   "sortsubs2_manual a [] = []" |
   "sortsubs2_manual a (x#xs) = insert a x (sortsubs2_manual a xs)"
 
-fun sortsubs2 :: "int list \<Rightarrow> int list \<Rightarrow> (int \<times> (nat \<times> nat)) list" where
+fun sortsubs2 :: "int list ⇒ int list ⇒ (int × (nat × nat)) list" where
   "sortsubs2 xs ys = sortsubs2_manual (mkArray xs ys) (subs xs ys)"
 
 value "sortsubs [1,2,3] [4,5]"  (* Expected result: [(- 4, 1, 2), (- 3, 1, 1), (- 3, 2, 2), (- 2, 2, 1), (- 2, 3, 2), (- 1, 3, 1)]*)
@@ -279,19 +321,19 @@ lemma sorstubs_sortsubs2:
 
 (*<----------------------- Divide and conquer ----------------------->*)
 
-fun incr :: "nat \<Rightarrow> (int \<times> (nat \<times> nat)) \<Rightarrow> (int \<times> (nat \<times> nat))" where
+fun incr :: "nat ⇒ (int × (nat × nat)) ⇒ (int × (nat × nat))" where
   "incr m (x, (i, j)) = (x, (i, m + j))"
 
-fun incl :: "nat \<Rightarrow> (int \<times> (nat \<times> nat)) \<Rightarrow> (int \<times> (nat \<times> nat))" where
+fun incl :: "nat ⇒ (int × (nat × nat)) ⇒ (int × (nat × nat))" where
   "incl m (x, (i, j)) = (x, (m + i, j))"
 
-fun incb :: "nat \<Rightarrow> (int \<times> (nat \<times> nat)) \<Rightarrow> (int \<times> (nat \<times> nat))" where
+fun incb :: "nat ⇒ (int × (nat × nat)) ⇒ (int × (nat × nat))" where
   "incb m (x, (i, j)) = (x, (m + i, m + j))"
 
-fun switch :: "(int \<times> (nat \<times> nat)) \<Rightarrow> (int \<times> (nat \<times> nat))" where
+fun switch :: "(int × (nat × nat)) ⇒ (int × (nat × nat))" where
   "switch (x, (i, j)) = (negate x, (j, i))"
 
-fun reverse :: "'a list \<Rightarrow> 'a list" where
+fun reverse :: "'a list ⇒ 'a list" where
   "reverse [] = []" |
   "reverse (x#xs) = reverse xs @ [x]"
   
